chore: use SMul rather than HMul in grind algebra typeclasses

src/Init/Grind/Module/Basic.lean
@@ -55,11 +55,11 @@ Use `IntModule` if the type has negation.
 -/
 class NatModule (M : Type u) extends AddCommMonoid M where
   /-- Scalar multiplication by natural numbers. -/
-  [nsmul : HMul Nat M M]
+  [nsmul : SMul Nat M]
   /-- Scalar multiplication by zero is zero. -/
-  zero_nsmul : ∀ a : M, 0 * a = 0
+  zero_nsmul : ∀ a : M, 0 • a = 0
   /-- Scalar multiplication by a successor. -/
-  add_one_nsmul : ∀ n : Nat, ∀ a : M, (n + 1) * a = n * a + a
+  add_one_nsmul : ∀ n : Nat, ∀ a : M, (n + 1) • a = n • a + a
 
 attribute [instance 100] NatModule.toAddCommMonoid NatModule.nsmul
 
@@ -71,17 +71,17 @@ Equivalently, an additive commutative group.
 -/
 class IntModule (M : Type u) extends AddCommGroup M where
   /-- Scalar multiplication by natural numbers. -/
-  [nsmul : HMul Nat M M]
+  [nsmul : SMul Nat M]
   /-- Scalar multiplication by integers. -/
-  [zsmul : HMul Int M M]
+  [zsmul : SMul Int M]
   /-- Scalar multiplication by zero is zero. -/
-  zero_zsmul : ∀ a : M, (0 : Int) * a = 0
+  zero_zsmul : ∀ a : M, (0 : Int) • a = 0
   /-- Scalar multiplication by one is the identity. -/
-  one_zsmul : ∀ a : M, (1 : Int) * a = a
+  one_zsmul : ∀ a : M, (1 : Int) • a = a
   /-- Scalar multiplication is distributive over addition in the integers. -/
-  add_zsmul : ∀ n m : Int, ∀ a : M, (n + m) * a = n * a + m * a
+  add_zsmul : ∀ n m : Int, ∀ a : M, (n + m) • a = n • a + m • a
   /-- Scalar multiplication by natural numbers is consistent with scalar multiplication by integers. -/
-  zsmul_natCast_eq_nsmul : ∀ n : Nat, ∀ a : M, (n : Int) * a = n * a
+  zsmul_natCast_eq_nsmul : ∀ n : Nat, ∀ a : M, (n : Int) • a = n • a
 
 attribute [instance 100] IntModule.toAddCommGroup IntModule.zsmul
 
@@ -174,33 +174,30 @@ namespace NatModule
 
 variable {M : Type u} [NatModule M]
 
-theorem one_nsmul (a : M) : 1 * a = a := by
+theorem one_nsmul (a : M) : 1 • a = a := by
   rw [← Nat.zero_add 1, add_one_nsmul, zero_nsmul, AddCommMonoid.zero_add]
 
-theorem add_nsmul (n m : Nat) (a : M) : (n + m) * a = n * a + m * a := by
+theorem add_nsmul (n m : Nat) (a : M) : (n + m) • a = n • a + m • a := by
   induction m with
   | zero => rw [Nat.add_zero, zero_nsmul, AddCommMonoid.add_zero]
   | succ m ih => rw [add_one_nsmul, ← Nat.add_assoc, add_one_nsmul, ih, AddCommMonoid.add_assoc]
 
-theorem nsmul_zero (n : Nat) : n * (0 : M) = 0 := by
+theorem nsmul_zero (n : Nat) : n • (0 : M) = 0 := by
   induction n with
   | zero => rw [zero_nsmul]
   | succ n ih => rw [add_one_nsmul, ih, AddCommMonoid.zero_add]
 
-theorem nsmul_add (n : Nat) (a b : M) : n * (a + b) = n * a + n * b := by
+theorem nsmul_add (n : Nat) (a b : M) : n • (a + b) = n • a + n • b := by
   induction n with
   | zero => rw [zero_nsmul, zero_nsmul, zero_nsmul, AddCommMonoid.zero_add]
   | succ n ih => rw [add_one_nsmul, add_one_nsmul, add_one_nsmul, ih, AddCommMonoid.add_assoc,
-      AddCommMonoid.add_left_comm (n * b), AddCommMonoid.add_assoc]
+      AddCommMonoid.add_left_comm (n • b), AddCommMonoid.add_assoc]
 
-theorem mul_nsmul (n m : Nat) (a : M) : (n * m) * a = n * (m * a) := by
+theorem mul_nsmul (n m : Nat) (a : M) : (n * m) • a = n • (m • a) := by
   induction n with
   | zero => simp [zero_nsmul]
   | succ n ih =>
     rw [Nat.add_one_mul, add_nsmul, ih, add_nsmul, one_nsmul]
-
-instance (priority := 100) (M : Type u) [NatModule M] : SMul Nat M where
-  smul a x := a * x
 
 end NatModule
 
@@ -208,45 +205,42 @@ namespace IntModule
 
 open NatModule AddCommGroup
 
-instance (priority := 100) (M : Type u) [IntModule M] : SMul Int M where
-  smul a x := a * x
-
 variable {M : Type u} [IntModule M]
 
-theorem neg_zsmul (n : Int) (a : M) : (-n) * a = - (n * a) := by
-  apply (add_left_inj (n * a)).mp
+theorem neg_zsmul (n : Int) (a : M) : (-n) • a = - (n • a) := by
+  apply (add_left_inj (n • a)).mp
   rw [← add_zsmul, Int.add_left_neg, zero_zsmul, neg_add_cancel]
 
-theorem zsmul_zero (n : Int) : n * (0 : M) = 0 := by
+theorem zsmul_zero (n : Int) : n • (0 : M) = 0 := by
   match n with
   | (n : Nat) => rw [zsmul_natCast_eq_nsmul, NatModule.nsmul_zero]
   | -(n + 1 : Nat) => rw [neg_zsmul, zsmul_natCast_eq_nsmul, NatModule.nsmul_zero, neg_zero]
 
-theorem zsmul_add (n : Int) (a b : M) : n * (a + b) = n * a + n * b := by
+theorem zsmul_add (n : Int) (a b : M) : n • (a + b) = n • a + n • b := by
   match n with
   | (n : Nat) => rw [zsmul_natCast_eq_nsmul, NatModule.nsmul_add, zsmul_natCast_eq_nsmul, zsmul_natCast_eq_nsmul]
   | -(n + 1 : Nat) => rw [neg_zsmul, zsmul_natCast_eq_nsmul, NatModule.nsmul_add,
       neg_zsmul, zsmul_natCast_eq_nsmul, neg_zsmul, zsmul_natCast_eq_nsmul, neg_add]
 
-theorem zsmul_neg (n : Int) (a : M) : n * (-a) = - (n * a) := by
-  apply (add_left_inj (n * a)).mp
+theorem zsmul_neg (n : Int) (a : M) : n • (-a) = - (n • a) := by
+  apply (add_left_inj (n • a)).mp
   rw [← zsmul_add, neg_add_cancel, neg_add_cancel, zsmul_zero]
 
-theorem zsmul_sub (k : Int) (a b : M) : k * (a - b) = k * a - k * b := by
+theorem zsmul_sub (k : Int) (a b : M) : k • (a - b) = k • a - k • b := by
   rw [sub_eq_add_neg, zsmul_add, zsmul_neg, ← sub_eq_add_neg]
 
-theorem sub_zsmul (k₁ k₂ : Int) (a : M) : (k₁ - k₂) * a = k₁ * a - k₂ * a := by
+theorem sub_zsmul (k₁ k₂ : Int) (a : M) : (k₁ - k₂) • a = k₁ • a - k₂ • a := by
   rw [Int.sub_eq_add_neg, add_zsmul, neg_zsmul, ← sub_eq_add_neg]
 
 private theorem mul_zsmul_aux (n : Nat) (m : Int) (a : M) :
-    ((n : Int) * m) * a = (n : Int) * (m * a) := by
+    ((n : Int) * m) • a = (n : Int) • (m • a) := by
   induction n with
   | zero => simp [zero_zsmul]
   | succ n ih =>
     rw [Int.natCast_add, Int.add_mul, add_zsmul, Int.natCast_one,
       Int.one_mul, add_zsmul, one_zsmul, ih]
 
-theorem mul_zsmul (n m : Int) (a : M) : (n * m) * a = n * (m * a) := by
+theorem mul_zsmul (n m : Int) (a : M) : (n * m) • a = n • (m • a) := by
   match n with
   | (n : Nat) => exact mul_zsmul_aux n m a
   | -(n + 1 : Nat) => rw [Int.neg_mul, neg_zsmul, mul_zsmul_aux, neg_zsmul]
@@ -264,7 +258,7 @@ and the theorem `eq_zero_of_mul_eq_zero`.)
 -/
 class NoNatZeroDivisors (α : Type u) [NatModule α] where
   /-- If `k * a ≠ k * b` then `k ≠ 0` or `a ≠ b`.-/
-  no_nat_zero_divisors : ∀ (k : Nat) (a b : α), k ≠ 0 → k * a = k * b → a = b
+  no_nat_zero_divisors : ∀ (k : Nat) (a b : α), k ≠ 0 → k • a = k • b → a = b
 
 export NoNatZeroDivisors (no_nat_zero_divisors)
 
@@ -272,7 +266,7 @@ namespace NoNatZeroDivisors
 
 /-- Alternative constructor for `NoNatZeroDivisors` when we have an `IntModule`. -/
 def mk' {α} [IntModule α]
-    (eq_zero_of_mul_eq_zero : ∀ (k : Nat) (a : α), k ≠ 0 → k * a = 0 → a = 0) :
+    (eq_zero_of_mul_eq_zero : ∀ (k : Nat) (a : α), k ≠ 0 → k • a = 0 → a = 0) :
     NoNatZeroDivisors α where
   no_nat_zero_divisors k a b h₁ h₂ := by
     rw [← AddCommGroup.sub_eq_zero_iff, ← IntModule.zsmul_natCast_eq_nsmul,
@@ -282,7 +276,7 @@ def mk' {α} [IntModule α]
     apply eq_zero_of_mul_eq_zero k (a - b) h₁ h₂
 
 theorem eq_zero_of_mul_eq_zero {α : Type u} [NatModule α] [NoNatZeroDivisors α] {k : Nat} {a : α}
-    : k ≠ 0 → k * a = 0 → a = 0 := by
+    : k ≠ 0 → k • a = 0 → a = 0 := by
   intro h₁ h₂
   replace h₁ : k ≠ 0 := by intro h; simp [h] at h₁
   exact no_nat_zero_divisors k a 0 h₁ (by rwa [NatModule.nsmul_zero])
